experiments/rupicola/Compiler.V2.SemanticTyping.fst
@@ -1,0 +1,165 @@
+module Compiler.V2.SemanticTyping
+
+open FStar.Tactics
+open FStar.Tactics.Typeclasses
+open FStar.Calc
+open FStar.List.Tot
+
+open STLC
+
+let rec elab_typ (t:typ) : Type0 =
+  match t with
+  | TUnit -> unit
+  | TArr t1 t2 -> (elab_typ t1 -> elab_typ t2)
+
+class compile_typ (s:Type) = {
+  [@@@no_method] t : (t:typ{elab_typ t == s}) // this could already create universe problems when using monads `Type u#a -> Type u#(max 1 a)`
+}
+
+instance compile_typ_unit : compile_typ unit = { t = TUnit }
+instance compile_typ_arrow s1 s2 {| c1:compile_typ s1 |} {| c2:compile_typ s2 |} : compile_typ (s1 -> s2) =
+  { t = begin
+    let t = (TArr c1.t c2.t) in
+    assert (elab_typ t == (elab_typ c1.t -> elab_typ c2.t))
+      by (norm [delta_only [`%elab_typ];zeta;iota]);
+    assert (s1 == elab_typ c1.t);
+    assert (s2 == elab_typ c2.t);
+    assert ((s1 -> s2) == elab_typ t) by (
+      rewrite (nth_binder (-1));
+      rewrite (nth_binder (-3))
+    );
+    t
+   end }
+
+// Some tests
+let test0 : compile_typ (unit) = solve
+let _ = assert (test0.t == TUnit)
+let test1 : compile_typ (unit -> unit) = solve
+let _ = assert (test1.t == (TArr TUnit TUnit))
+let test2 : compile_typ ((unit -> unit) -> (unit -> unit)) = solve
+let _ = assert (test2.t == TArr (TArr TUnit TUnit) (TArr TUnit TUnit))
+
+type env_card (g:env) =
+  g_card:nat{forall (i:nat). i < g_card ==> Some? (g i)}
+
+class compile_exp (#a:Type0) {| ca: compile_typ a |} (s:a) (g:env) (g_card:env_card g) = {
+  [@@@no_method] t : exp;
+  [@@@no_method] proof : unit -> Lemma (sem_typing g t ca.t)
+}
+
+assume val get_v : i:nat -> a:Type -> a
+(** CA: this is an abstraction that helps with dealing with variables.
+   It is like a symbol we introduce when dealing with lambdas and eliminate when dealing with variables **)
+
+instance compile_exp_unit g card_g : compile_exp #unit #compile_typ_unit () g card_g = {
+  t = EUnit;
+  proof = (fun () -> assert (sem_typing g EUnit TUnit) by (explode ()));
+}
+
+let test_unit g n : compile_exp () g n = solve
+
+instance compile_exp_var (#a:Type) {| ca: compile_typ a |} g (g_card:env_card g) (i:nat{i < g_card /\ Some?.v (g (g_card-i-1)) == ca.t}) : compile_exp (get_v i a) g g_card =
+  let v = g_card-i-1 in {
+    t = EVar v;
+    proof = (fun () ->
+      assert (sem_typing g (EVar v) ca.t) by (explode ())
+    )
+  }
+
+instance compile_exp_lambda
+  g
+  (g_card:env_card g)
+  (#a:Type) {| ca: compile_typ a |}
+  (#b:Type) {| cb: compile_typ b |}
+  (f:a -> b) {| cf: (compile_exp #_ #cb (f (get_v g_card a)) (extend ca.t g) (g_card+1)) |}
+  : compile_exp #_ #solve (fun x -> f x) g g_card = {
+  t = ELam ca.t cf.t;
+  proof = (fun () ->
+    cf.proof ();
+    introduce forall (s:subfun g). wb_expr (TArr ca.t cb.t) (subst s (ELam ca.t cf.t)) with begin
+      assert (wb_expr (TArr ca.t cb.t) (subst s (ELam ca.t cf.t)) <==> wb_expr (TArr ca.t cb.t) (ELam ca.t (subst (sub_elam s) cf.t)));
+      assume ( (** CA: refl **)
+        wb_value (TArr ca.t cb.t) (ELam ca.t (subst (sub_elam s) cf.t)) ==>
+        wb_expr (TArr ca.t cb.t) (ELam ca.t (subst (sub_elam s) cf.t)));
+      introduce forall v. wb_value ca.t v ==>  wb_expr cb.t (subst (sub_beta v) (subst (sub_elam s) cf.t)) with begin
+        introduce _ ==> _ with _. begin
+            assume ((subst (sub_beta v) (subst (sub_elam s) cf.t)) ==
+                    (subst (subfun_extend s ca.t v ()) cf.t)) (** CA: substitution lemma *)
+        end
+      end
+    end
+  );
+}
+
+let test1_exp : compile_exp #(unit -> unit) (fun x -> ()) empty 0 =
+  solve
+let _ = assert (test1_exp.t == ELam TUnit (EUnit))
+
+let test2_exp : compile_exp #(unit -> unit) (fun x -> x) empty 0 =
+  solve
+let _ = assert (test2_exp.t == ELam TUnit (EVar 0))
+
+let test3_exp : compile_exp #(unit -> unit -> unit) (fun x y -> x) empty 0 =
+  solve
+let _ = assert (test3_exp.t == ELam TUnit (ELam TUnit (EVar 1)))
+
+let test4_exp : compile_exp #(unit -> unit -> unit) (fun x y -> y) empty 0 =
+  solve
+let _ = assert (test4_exp.t == ELam TUnit (ELam TUnit (EVar 0)))
+
+instance compile_exp_app
+  g
+  (g_card:env_card g)
+  (#a:Type) {| ca: compile_typ a |}
+  (#b:Type) {| cb: compile_typ b |}
+  (f:a -> b) {| cf: compile_exp #_ #solve f g g_card |}
+  (x:a)     {| cx: compile_exp #_ #ca x g g_card |}
+  : compile_exp #_ #cb (f x) g g_card = {
+  t = EApp (cf.t) (cx.t);
+  proof = (fun () ->
+    cf.proof ();
+    cx.proof ();
+    assert (forall (s:subfun g). wb_expr (TArr ca.t cb.t) (subst s cf.t));
+    assert (forall (s:subfun g). wb_expr ca.t (subst s cx.t));
+    assert (forall (s:subfun g) x' f'. is_value x' ==> is_value f' ==>
+      steps (subst s cf.t) (ELam ca.t f') ==>
+      steps (subst s cx.t) x'
+      ==> wb_expr cb.t (subst (sub_beta x') f')) by (
+      explode ()
+      );
+    assert (forall (s:subfun g) x' f'. is_value x' ==> is_value f' ==>
+      steps (subst s cf.t) (ELam ca.t f') ==>
+      steps (subst s cx.t) x'
+      ==> (forall (e':exp). steps (subst (sub_beta x') f') e' ==> irred e' ==> wb_value cb.t e'));
+    assume (forall (s:subfun g) e'. steps (EApp (subst s cf.t) (subst s cx.t)) e' ==> irred e' ==>
+      wb_value cb.t e');
+    assert (forall (s:subfun g). wb_expr cb.t (EApp (subst s cf.t) (subst s cx.t)));
+//    by (explode (); dump "H"  );
+    assert (forall (s:subfun g). wb_expr cb.t (subst s (EApp cf.t cx.t)));
+    assert (sem_typing g (EApp cf.t cx.t) cb.t))
+}
+
+let test0_fapp : compile_exp #unit #solve ((fun x y -> y) () ()) empty 0 =
+  solve
+let _ = assert (test0_fapp.t == EUnit)
+
+(** How to deal with top level definitions? **)
+
+val myf : unit -> unit
+let myf () = ()
+
+(* It seems that it just unfolds the definition of myf, which is pretty cool **)
+let test1_topf : compile_exp (myf ()) empty 0 =
+  solve
+// because of partial evaluation we have to consider both cases
+let _ = assert (test1_topf.t == EApp (ELam TUnit EUnit) EUnit \/
+                test1_topf.t == EUnit)
+
+val myf2 : unit -> unit -> unit
+let myf2 x y = x
+
+(* Also handles partial application. Pretty amazing! *)
+let test2_topf : compile_exp (myf2 ()) empty 0 =
+  solve
+let _ = assert (test2_topf.t == EApp (ELam TUnit (ELam TUnit (EVar 1))) EUnit \/
+                test2_topf.t == ELam TUnit EUnit)
